new-semantics/coq/events/Defs.v
@@ -417,26 +417,6 @@ Proof.
   des_ifs; eqb2eq loc; clarify.
 Qed.
 
-Definition remove {loc T} `{Eq loc} (f : loc -> option T) ℓ ℓ_param :=
-  if eqb ℓ ℓ_param then None else f ℓ_param.
-
-Notation "f '!!' ℓ" := (remove f ℓ)
-  (at level 100, ℓ at next level, right associativity).
-
-Lemma remove_assoc {loc T} `{Eq loc} (f : loc -> option T) ℓ ℓ' x :
-  ((f !! ℓ) !! ℓ') x = ((f !! ℓ') !! ℓ) x.
-Proof.
-  ii. unfold remove. des_ifs.
-Qed.
-
-Lemma remove_update_assoc {loc T} `{Eq loc} (f : loc -> option T) ℓ ν ℓ' x :
-  ℓ <> ν ->
-  ((ℓ !-> ℓ' ; f) !! ν) x = (ℓ !-> ℓ' ; f !! ν) x.
-Proof.
-  ii. unfold remove, update.
-  des_ifs. eqb2eq loc. clarify.
-Qed.
-
 Definition swap {loc T} `{Eq loc} (f : loc -> T) ℓ ν x :=
   if eqb x ℓ then f ν else if eqb x ν then f ℓ else f x.
 
