new-semantics/coq/playground/PMap.v
@@ -1,0 +1,458 @@
+(** * The extensional binary tries based on a canonical representation *)
+
+(* Authors: Andrew W. Appel, Princeton University,
+            Xavier Leroy, Collège de France and Inria.
+Copyright: Andrew W. Appel and Inria.
+   License: BSD-3-Clause. *)
+
+From Coq Require Import PArith.
+
+(* To avoid useless definitions of inductors in extracted code. *)
+Local Unset Elimination Schemes.
+Local Unset Case Analysis Schemes.
+
+Set Implicit Arguments.
+
+Class map {K V} := mkMap {
+rep : Type;
+
+(* fundamental operation, all others are axiomatized in terms of this one *)
+  get: rep -> K -> option V;
+
+  empty : rep;
+  put : rep -> K -> V -> rep;
+  remove : rep -> K -> rep;
+
+  (* R is the type of the accumulator *)
+  fold {R: Type} : (R -> K -> V -> R) -> R -> rep -> R;
+}.
+
+Arguments map : clear implicits.
+Global Coercion rep : map >-> Sortclass.
+Global Hint Mode map + + : typeclass_instances.
+Local Hint Mode map - - : typeclass_instances.
+
+Class ok {K V : Type} {map : map K V}: Prop := {
+  map_ext : forall m1 m2, (forall k, get m1 k = get m2 k) -> m1 = m2;
+  get_empty : forall k, get empty k = None;
+  get_put_same : forall m k v, get (put m k v) k = Some v;
+  get_put_diff : forall m k v k', k <> k' -> get (put m k' v) k = get m k;
+  get_remove_same : forall m k, get (remove m k) k = None;
+  get_remove_diff : forall m k k', k <> k' -> get (remove m k') k = get m k;
+  fold_spec{R: Type} : forall (P: rep -> R -> Prop) (f: R -> K -> V -> R) r0,
+      P empty r0 ->
+      (forall k v m r, get m k = None -> P m r -> P (put m k v) (f r k v)) ->
+      forall m, P m (fold f r0 m);
+  (* Folding over a map preserves relations: *)
+  fold_parametricity: forall {A B : Type} (R : A -> B -> Prop)
+                             (fa: A -> K -> V -> A) (fb: B -> K -> V -> B),
+      (forall a b k v, R a b -> R (fa a k v) (fb b k v)) ->
+      forall a0 b0, R a0 b0 -> forall m, R (fold fa a0 m) (fold fb b0 m);
+}.
+Arguments ok {_ _} _.
+
+Module PTree.
+
+(** ** Representation of tries *)
+
+(** The type [tree'] of nonempty tries *)
+Inductive tree' {V : Type} : Type :=
+  (* this node is nonempty *)
+  | NodeM (v : V) (l r : option tree')
+  (* this node is empty, the first nonempty subtrie is the left one *)
+  | Node0 (l : tree') (r : option tree')
+  (* this node is empty, the first nonempty subtrie is the right one *)
+  | Node1 (r : tree')
+.
+
+Arguments tree' : clear implicits.
+
+Definition tree V := option (tree' V).
+
+Section TREE_IND.
+  Context {V : Type}.
+  Context (P : tree V -> Prop) (P' : tree' V -> Prop).
+  Context (PNodeM : forall v l r, P l -> P r -> P' (NodeM v l r))
+          (PNode0 : forall l r, P' l -> P r -> P' (Node0 l r))
+          (PNode1 : forall r, P' r -> P' (Node1 r))
+          (PNone : P None)
+          (PSome : forall t', P' t' -> P (Some t')).
+
+  Fixpoint _tree'_ind t' : P' t' :=
+  let _tree_ind ot : P ot :=
+    match ot with
+    | None => PNone
+    | Some t => PSome (_tree'_ind t)
+    end
+  in match t' with
+  | NodeM v l r => PNodeM v (_tree_ind l) (_tree_ind r)
+  | Node0 l' r => PNode0 (_tree'_ind l') (_tree_ind r)
+  | Node1 r' => PNode1 (_tree'_ind r')
+  end.
+End TREE_IND.
+
+Definition tree'_ind {V} (P' : tree' V -> Prop) PNodeM PNode0 PNode1 :=
+  let P t := match t with None => True | Some t' => P' t' end in
+  _tree'_ind P P' PNodeM PNode0 PNode1 I ltac:(auto).
+
+(** A smart constructor.  Given a (possibly empty) left subtree,
+    a (possibly absent) value, and a (possibly empty) right subtree,
+    it builds the corresponding tree. *)
+
+Definition Node {V} (l: tree V) (o: option V) (r: tree V) : tree V :=
+  match l,o,r with
+  | None, None, None => None
+  | _, Some v, _ => Some (NodeM v l r)
+  | Some l', None, _ => Some (Node0 l' r)
+  | None, None, Some r' => Some (Node1 r')
+  end.
+
+(** ** Basic operations: [empty], [get], [set], [remove], [fold] *)
+
+Definition empty (V : Type) : tree V := None.
+
+(** Operations such as [get] follow a common pattern:
+    first, a recursive function [get'] over nonempty tries;
+    then, a non-recursive function [get] to handle empty tries too. *)
+
+Local Open Scope positive_scope.
+
+Fixpoint get' {V} (p : positive) (m : tree' V) : option V :=
+  match p, m with
+  | 1, NodeM v _ _ => Some v
+  | 1, _ => None
+  | q~0, NodeM _ (Some l) _
+  | q~0, Node0 l _ => get' q l
+  | q~0, _ => None
+  | q~1, NodeM _ _ (Some r)
+  | q~1, Node0 _ (Some r)
+  | q~1, Node1 r => get' q r
+  | q~1, _ => None
+  end.
+
+Definition get {V} (p : positive) (m : tree V) : option V :=
+  match m with
+  | None => None
+  | Some m' => get' p m'
+  end.
+
+(** [set0 p v] constructs the singleton trie that maps [p] to [v]
+    and has no other bindings. *)
+
+Fixpoint set0 {V} (p : positive) (v : V) : tree' V :=
+  match p with
+  | 1 => NodeM v None None
+  | q~0 => Node0 (set0 q v) None
+  | q~1 => Node1 (set0 q v)
+  end.
+
+Fixpoint set' {V} (p : positive) (v : V) (m : tree' V) : tree' V :=
+  let set p v m :=
+    match m with
+    | None => set0 p v
+    | Some m' => set' p v m'
+    end
+  in match p, m with
+  | 1, NodeM _ l r => NodeM v l r
+  | 1, Node0 l r => NodeM v (Some l) r
+  | 1, Node1 r => NodeM v None (Some r)
+  | q~0, NodeM w l r => NodeM w (Some (set q v l)) r
+  | q~0, Node0 l r => Node0 (set' q v l) r
+  | q~0, Node1 r => Node0 (set0 q v) (Some r)
+  | q~1, NodeM w l r => NodeM w l (Some (set q v r))
+  | q~1, Node0 l r => Node0 l (Some (set q v r))
+  | q~1, Node1 r => Node1 (set' q v r)
+  end.
+
+Definition put {V} p v (m : tree V) :=
+  match m with
+  | None => set0 p v
+  | Some m' => set' p v m'
+  end.
+
+Fixpoint remove' {V} (p : positive) (m : tree' V) : tree V :=
+  let remove p m :=
+    match m with
+    | None => None
+    | Some m' => remove' p m'
+    end
+  in match p, m with
+  | 1, NodeM _ None None => None
+  | 1, NodeM _ (Some l) r => Some (Node0 l r)
+  | 1, NodeM _ None (Some r) => Some (Node1 r)
+  | 1, _ => Some m
+  | q~0, NodeM v l r => Node (remove q l) (Some v) r
+  | q~0, Node0 l r => Node (remove' q l) None r
+  | q~0, _ => Some m
+  | q~1, NodeM v l r => Node l (Some v) (remove q r)
+  | q~1, Node0 l r => Node (Some l) None (remove q r)
+  | q~1, Node1 r => Node None None (remove' q r)
+  end.
+
+(* k : positive -> positive *)
+Fixpoint fold'' {R V : Type}
+  (f : R -> positive -> V -> R) (acc : R) k (m' : tree' V) : R :=
+  let fold' f acc k m :=
+    match m with
+    | None => acc
+    | Some m' => fold'' f acc k m'
+    end
+  in match m' with
+  | NodeM v l r =>
+    let accl := fold' f acc (fun x => k (x~0)) l in
+    let accv := f accl (k 1) v in
+    fold' f accv (fun x => k (x~1)) r
+  | Node0 l r =>
+    let accl := fold'' f acc (fun x => k (x~0)) l in
+    fold' f accl (fun x => k (x~1)) r
+  | Node1 r => fold'' f acc (fun x => k (x~1)) r
+  end.
+
+Local Close Scope positive_scope.
+
+(** ** Good variable properties for the basic operations *)
+
+Theorem get_empty :
+  forall (V : Type) (i : positive), get i (empty V) = None.
+Proof. reflexivity. Qed.
+
+Lemma gss0: forall {V} p (x : V), get' p (set0 p x) = Some x.
+Proof. induction p; simpl; auto. Qed.
+
+Lemma gso0: forall {V} p q (x : V), p <> q -> get' p (set0 q x) = None.
+Proof.
+  induction p; destruct q; simpl; intros; auto; try apply IHp; congruence.
+Qed.
+
+Lemma gss V (m' : tree' V) :
+  forall i x, get' i (set' i x m') = Some x.
+Proof with auto using gss0.
+  induction m' using tree'_ind; intros; destruct i; simpl ...
+  - destruct r ...
+  - destruct l ...
+  - destruct r ...
+Qed.
+
+Lemma gso V (m' : tree' V) :
+  forall i j x, i <> j -> get' i (set' j x m') = get' i m'.
+Proof with auto using gso0.
+  induction m' using tree'_ind;
+  intros; destruct i, j; simpl; try contradiction ...
+  all: assert (i <> j) by congruence ...
+  - destruct r ...
+  - destruct l ...
+  - destruct r ...
+Qed.
+
+Lemma gNode :
+  forall {V} (i: positive) (l: tree V) (x: option V) (r: tree V),
+  get i (Node l x r) = match i with xH => x | xO j => get j l | xI j => get j r end.
+Proof.
+  intros. destruct l, x, r; simpl; auto; destruct i; auto.
+Qed.
+
+Local Opaque Node.
+
+Lemma grs V (m' : tree' V) :
+  forall i, get i (remove' i m') = None.
+Proof with (try rewrite gNode; auto).
+  induction m' using tree'_ind; intros; destruct i; simpl ...
+  - destruct r ...
+  - destruct l ...
+  - destruct l ... destruct r ...
+  - destruct r ...
+Qed.
+
+Lemma gro V (m' : tree' V) :
+  forall i j, i <> j -> get i (remove' j m') = get' i m'.
+Proof with (try rewrite gNode; auto).
+  induction m' using tree'_ind;
+  intros; destruct i, j; simpl; try contradiction ...
+  all: try assert (i <> j) by congruence ...
+  - destruct r ...
+  - destruct l ... destruct r ...
+  - destruct l ...
+  - destruct l ... destruct r ...
+  - destruct r ...
+Qed.
+
+Lemma fold''_spec {R V : Type} :
+  forall (P : tree V -> R -> Prop) (f : R -> positive -> V -> R) acc k
+    (PEmpty : P None acc)
+    (PNodes : forall i v m r, get i m = None -> P m r -> P (Some (put i v m)) (f r (k i) v)),
+    forall m, P (Some m) (fold'' f acc k m).
+Proof.
+  intros. generalize dependent P. revert f acc k.
+  induction m using tree'_ind; intros; simpl;
+  set (P0 t := match t with None => P None | Some t' => P (Some (Node0 t' None)) end);
+  set (P1 t := match t with None => P None | Some t' => P (Some (Node1 t')) end).
+  Local Ltac appnodes PNodes :=
+  match goal with
+  | |- _ (Some (?N (set' ?i _ ?l) ?r)) (_ _ (_ (?x ?i)) _) =>
+    apply PNodes with (m := Some (N l r)) (i := x i); auto
+  | |- _ (Some (?N (set0 ?i _) ?r)) (_ _ (_ (?x ?i)) _) =>
+    apply PNodes with (m := r) (i := x i); auto
+  | |- _ (Some (?N (set' _ _ ?l))) (_ _ (_ (?x ?i)) _) =>
+    apply PNodes with (m := Some (N l)) (i := x i); auto
+  | |- _ (Some (?N (set0 _ _))) (_ _ (_ (?x ?i)) _) =>
+    apply PNodes with (m := None) (i := x i); auto
+  | |- _ (Some _) (_ _ (_ xH) _) =>
+    apply PNodes with (m := None) (i := xH); auto
+  | |- _ (Some (?N ?v ?l (Some (_ _ _ ?r)))) (_ _ (_ (?x ?i)) _) =>
+    apply PNodes with (m := Some (N v l r)) (i := (x i)); auto
+  | |- _ (Some (?N ?l (Some (_ _ _ ?r)))) (_ _ (_ (?x ?i)) _) =>
+    apply PNodes with (m := Some (N l r)) (i := (x i)); auto
+  end.
+  - assert (forall (v : V) (a b : tree V),
+      NodeM v a b = put 1 v (Node a None b)) as RR by (destruct a, b; auto).
+    rewrite RR.
+    destruct r; try apply H0;
+    solve [
+      intros; rewrite <- RR in *; appnodes PNodes |
+      destruct l; apply PNodes; auto;
+      apply H with (P := P0); auto;
+      intros ? ? [? |] ? ? ?; subst P0; simpl; appnodes PNodes
+    ].
+  - destruct r; try apply H;
+    solve [
+      intros; appnodes PNodes |
+      apply IHm with (P := P0); auto;
+      intros ? ? [? |] ? ? ?; subst P0; simpl; appnodes PNodes
+    ].
+  - apply IHm with (P := P1); auto.
+    intros ? ? [t' |] ? ? ?; simpl; appnodes PNodes.
+Qed.
+
+Lemma fold''_parametricity {A B V : Type} :
+  forall (R : A -> B -> Prop) (fa: A -> positive -> V -> A) (fb: B -> positive -> V -> B)
+    (RApp : forall a b i v (REL : R a b), R (fa a i v) (fb b i v)),
+  forall m a0 b0 k (RAcc : R a0 b0),
+    R (fold'' fa a0 k m) (fold'' fb b0 k m).
+Proof.
+  do 4 intro.
+  induction m using tree'_ind; intros;
+  [destruct l, r | destruct r |]; eauto.
+Qed.
+
+Lemma tree'_nonempty {V} (m : tree' V) :
+  exists k, get' k m <> None.
+Proof.
+  induction m using tree'_ind;
+  [destruct l, r | destruct r|];
+  repeat match goal with
+  | H : exists _, _ |- _ =>
+    let k := fresh "k" in destruct H as [k H];
+    try solve [exists (xO k); eauto | exists (xI k); eauto]
+  end; exists xH; intro EQ; inversion EQ.
+Qed.
+
+Lemma tree'_contradiction {V} (m : tree' V) :
+  ~ forall k, get' k m = None.
+Proof.
+  destruct (tree'_nonempty m) as (k & ?). auto.
+Qed.
+
+Lemma tree_empty {V} (m : tree V) :
+  (forall k, get k m = None) -> m = None.
+Proof.
+  destruct m; intros; simpl in *; auto.
+  exfalso. eapply tree'_contradiction; eauto.
+Qed.
+
+Lemma map_ext {V} (m1 : tree' V) :
+  forall m2 (EQ : forall k, get' k m1 = get' k m2),
+    m1 = m2.
+Proof.
+  induction m1 using tree'_ind; intros; destruct m2;
+  match goal with
+  | |- NodeM ?v ?l ?r = NodeM ?v' ?l' ?r' =>
+    assert (v = v') by
+      (specialize (EQ xH); inversion EQ; auto);
+    assert (forall k, get k l = get k l') by
+      (intros; specialize (EQ (xO k)); eauto);
+    assert (forall k, get k r = get k r') by
+      (intros; specialize (EQ (xI k)); eauto);
+    f_equal
+  | |- Node0 ?l ?r = Node0 ?l' ?r' =>
+    assert (forall k, get' k l = get' k l') by
+      (intros; specialize (EQ (xO k)); eauto);
+    assert (forall k, get k r = get k r') by
+      (intros; specialize (EQ (xI k)); eauto);
+    f_equal
+  | |- Node1 ?r = Node1 ?r' =>
+    assert (forall k, get' k r = get' k r') by
+      (intros; specialize (EQ (xI k)); eauto);
+    f_equal
+  | _ => solve [specialize (EQ xH); inversion EQ]
+  | |- context [Node0 ?m _] =>
+    destruct (tree'_nonempty m) as (k & ?);
+    specialize (EQ (xO k)); simpl in EQ;
+    rewrite EQ in *; contradiction
+  end; eauto;
+  match goal with
+  | |- ?a = ?b =>
+    destruct a, b; simpl in *; auto; [
+    f_equal; eauto |
+    exfalso; eapply tree'_contradiction; eauto |
+    symmetry; apply tree_empty; eauto]
+  end.
+Qed.
+End PTree.
+
+(* from stdpp/strings.v *)
+From Coq Require Import Ascii.
+From Coq Require Export String.
+
+Local Definition funapp {A B} (f : A -> B) (x : A) := f x.
+#[local] Infix "$" := funapp (at level 60, right associativity).
+Local Definition bool_cons_pos (b : bool) (p : positive) : positive :=
+  if b then xI p else xO p.
+Local Definition ascii_cons_pos (c : ascii) (p : positive) : positive :=
+  match c with
+  | Ascii b0 b1 b2 b3 b4 b5 b6 b7 =>
+     bool_cons_pos b0 $ bool_cons_pos b1 $ bool_cons_pos b2 $
+       bool_cons_pos b3 $ bool_cons_pos b4 $ bool_cons_pos b5 $
+       bool_cons_pos b6 $ bool_cons_pos b7 p
+  end.
+
+Fixpoint string_to_pos (s : string) : positive :=
+  match s with
+  | EmptyString => 1
+  | String c s => ascii_cons_pos c (string_to_pos s)
+  end.
+
+(* The decoder that turns [positive] into string results in 256 cases (we need
+to peel off 8 times a [~0]/[~1] constructor) and a number of fall through cases.
+We avoid writing these cases explicitly by generating the definition using Ltac.
+The lemma [string_of_to_pos] ensures the generated definition is correct.
+
+Alternatively, we could implement it in two steps. Convert the [positive] to
+[list bool], and convert the list to [string]. This definition will be slower
+since auxilary data structures are created. *)
+Local Fixpoint pos_to_string (p : positive) : string.
+Proof.
+  (** The argument [p] is the [positive] that we are peeling off.
+  The argument [a] is the constructor [Ascii] partially applied to some number
+  of Booleans (so its Coq type changes during the iteration).
+  The argument [n] says how many more Booleans are needed to make this fully
+  applied so that the [constr] has type ascii. *)
+  let rec gen p a n :=
+    lazymatch n with
+    (* This character is done. Stop the ltac recursion; recursively invoke
+    [pos_to_string] on the Gallina level for the remaining bits. *)
+    | 0 => exact (String a (pos_to_string p))
+    (* There are more bits to consume for this character, generate an
+    appropriate [match] with ltac. *)
+    | S ?n =>
+       exact (match p with
+              | 1 => EmptyString
+              | p~0 => ltac:(gen p (a false) n)
+              | p~1 => ltac:(gen p (a true) n)
+              end%positive)
+    end in
+  gen p Ascii 8.
+Defined.
+
+Local Lemma pos_to_string_string_to_pos s : pos_to_string (string_to_pos s) = s.
+Proof. induction s as [|[[][][][][][][][]]]; simpl; f_equal; first [reflexivity | assumption]. Qed.
+
